theories/util/functional_choice.v
@@ -1,0 +1,3 @@
+Require Import ChoiceFacts.
+
+Axiom inhabited_forall_commute: InhabitedForallCommute.
